BinaryHeap/CompleteTree/Lemmas.lean
@@ -31,6 +31,14 @@ theorem CompleteTree.right_unfold {α : Type u} {o p : Nat} (v : α) (l : Comple
 
 theorem CompleteTree.contains_unfold {α : Type u} {o p : Nat} (element : α) (v : α) (l : CompleteTree α o) (r : CompleteTree α p) (h₁ : p ≤ o) (h₂ : o < 2 * (p + 1)) (h₃ : (o + 1).isPowerOfTwo ∨ (p + 1).isPowerOfTwo) : (CompleteTree.branch v l r h₁ h₂ h₃).contains element = (v=element ∨ l.contains element ∨ r.contains element) := rfl
 
+theorem CompleteTree.contains_as_root_left_right {α : Type u} {n : Nat} (tree : CompleteTree α n) (element : α) (h₁ : n > 0) : tree.contains element = (tree.root h₁ = element ∨ (tree.left h₁).contains element ∨ (tree.right h₁).contains element) := by
+  unfold root
+  match n, tree with
+  | (_+_), .branch v l r _ _ _=>
+    simp[left_unfold, right_unfold]
+    rfl
+
+
 theorem CompleteTree.heqSameLeftLen {α : Type u} {n m : Nat} {a : CompleteTree α n} {b : CompleteTree α m} (h₁ : n = m) (h₂ : n > 0) (h₃ : HEq a b) : a.leftLen h₂ = b.leftLen (h₁.subst h₂) := by
   subst n
   have h₃ : a = b := eq_of_heq h₃
@@ -43,6 +51,12 @@ theorem CompleteTree.heqSameRightLen {α : Type u} {n m : Nat} {a : CompleteTree
 
 theorem CompleteTree.heqSameRoot {α : Type u} {n m : Nat} {a : CompleteTree α n} {b : CompleteTree α m} (h₁ : n = m) (h₂ : n > 0) (h₃ : HEq a b) : a.root h₂ = b.root (h₁.subst h₂) := by
   subst n
+  have h₃ : a = b := eq_of_heq h₃
+  congr
+
+theorem CompleteTree.heqContains {α : Type u} {n m : Nat} {a : CompleteTree α n} {b : CompleteTree α m} (h₁ : n = m) (h₃ : HEq a b) : ∀(v : α), a.contains v = b.contains v := by
+  intro value
+  subst m
   have h₃ : a = b := eq_of_heq h₃
   congr
 
